IO.thy
@@ -132,6 +132,7 @@ lemma bind_assoc:
   by(simp add: IO.bind_def Abs_io_inverse Abs_io_inject fun_eq_iff split: prod.splits)
 
 
+subsection\<open>Code Generator Setup\<close>
 text \<open>
   We don't expose our \<^const>\<open>IO.bind\<close> definition to code.
   We use the built-in definitions of the target language (e.g., Haskell, SML).
@@ -156,7 +157,7 @@ text\<open>
 code_printing type_constructor io \<rightharpoonup> (Haskell) "Prelude.IO _"
                                      and (SML) "unit -> _"
 
-subsection\<open>Code Generator Setup and Basic Functions\<close>
+
 text\<open>
 In Isabelle, a \<^typ>\<open>string\<close> is just a type synonym for \<^typ>\<open>char list\<close>.
 When translating a \<^typ>\<open>string\<close> to Haskell, Isabelle does not use Haskell's \<^verbatim>\<open>String\<close> or 
@@ -223,5 +224,49 @@ lemma "do { _ \<leftarrow> println (STR ''foo'');
             println (STR ''bar'')} =
       println (STR ''foo'') \<then> (println (STR ''bar''))"
   by simp
+
+
+
+subsection\<open>Modelling Running an \<^typ>\<open>'\<alpha> io\<close> Function\<close>
+text\<open>
+  Apply some function \<^term>\<open>iofun :: '\<alpha> io\<close> to a specific world and return the new world
+  (discarding the result of \<^term>\<open>iofun\<close>).
+\<close>
+definition exec :: "'\<alpha> io \<Rightarrow> \<^url> \<Rightarrow> \<^url>" where
+  "exec iofun world = snd (Rep_io iofun world)"
+
+text\<open>Similar, but only get the result.\<close>
+definition eval :: "'\<alpha> io \<Rightarrow> \<^url> \<Rightarrow> '\<alpha>" where
+  "eval iofun world = fst (Rep_io iofun world)"
+
+text\<open>
+  Essentially, \<^const>\<open>exec\<close> and \<^const>\<open>eval\<close> extract the payload \<^typ>\<open>'\<alpha>\<close> and \<^typ>\<open>\<^url>\<close>
+  when executing an \<^typ>\<open>'\<alpha> io\<close>.
+\<close>
+lemma "Abs_io (\<lambda>world. (eval iofun world, exec iofun world)) = iofun"
+  by(simp add: exec_def eval_def Rep_io_inverse)
+
+lemma exec_Abs_io: "exec (Abs_io f) world = snd (f world)"
+  by(simp add: exec_def Abs_io_inverse)
+
+
+lemma exec_then:
+    "exec (io\<^sub>1 \<then> io\<^sub>2) world = exec io\<^sub>2 (exec io\<^sub>1 world)"
+  and eval_then:
+    "eval (io\<^sub>1 \<then> io\<^sub>2) world = eval io\<^sub>2 (exec io\<^sub>1 world)"
+  by (simp_all add: exec_def eval_def bind_def Abs_io_inverse split_beta)
+
+lemma exec_bind:
+    "exec (io\<^sub>1 \<bind> io\<^sub>2) world = exec (io\<^sub>2 (eval io\<^sub>1 world)) (exec io\<^sub>1 world)"
+  and eval_bind:
+    "eval (io\<^sub>1 \<bind> io\<^sub>2) world = eval (io\<^sub>2 (eval io\<^sub>1 world)) (exec io\<^sub>1 world)"
+  by(simp_all add: exec_def eval_def bind_def Abs_io_inverse split_beta)
+
+lemma exec_return:
+    "exec (IO.return a) world = world"
+  and
+    "eval (IO.return a) world = a"
+  by (simp_all add: exec_def eval_def Abs_io_inverse return_def)
+
 
 end
